PDG.dfy
@@ -3,13 +3,33 @@ include "Util.dfy"
 include "CFG.dfy"
 
 // PDG Definitions:
-datatype Tag = Control | Data(vars: set<Variable>)
+
+//datatype Tag = Control | Data(vars: set<Variable>)
+datatype Tag = Control | Data(v: Variable) // changed to singleton variable
 datatype PDGNode = Node(l:Label) | Entry
 type PDGEdge = (PDGNode, PDGNode, Tag)
+type PDG = (set<PDGNode>, set<PDGEdge>, map<CFGNode, PDGNode>)
 
-method ComputePDG(S: Statement, cfg: CFG) returns (N: set<PDGNode>, E: set<PDGEdge>)
+//method ComputePDG(S: Statement, cfg: CFG) returns (N: set<PDGNode>, E: set<PDGEdge>)
+
+
+method ComputePDG(S: Statement, cfg: CFG) returns (pdg: PDG)
 {
-	var cfgToPdgNodeMap : map<CFGNode, PDGNode> := map[];
+	var nodes, cfgToPdgNodeMap := ComputePDGNodes(S, cfg);
+	var edges := ComputePDGEdges(S, cfg, cfgToPdgNodeMap);
+
+	var pdg := (nodes, edges, cfgToPdgNodeMap);
+}
+
+function PDGEdges(S: Statement, cfg: CFG, cfgToPdgNodeMap: map<CFGNode, PDGNode>): set<PDGEdge>
+{
+	//set edge: PDGEdge | edge.0
+}
+
+
+method ComputePDGNodes(S: Statement, cfg: CFG) returns (N: set<PDGNode>, cfgToPdgNodeMap: map<CFGNode, PDGNode>)
+{
+	cfgToPdgNodeMap := map[];
 	N := {};
 	var cfgNodes := cfg.0;
 	while (|cfgNodes| > 0) {
@@ -26,10 +46,15 @@ method ComputePDG(S: Statement, cfg: CFG) returns (N: set<PDGNode>, E: set<PDGEd
 				N := N + {pdgNode};
 				cfgToPdgNodeMap := cfgToPdgNodeMap[cfgNode := pdgNode];
 			case Exit =>
+
 		}
 	}
+}
+
+method ComputePDGEdges(S: Statement, cfg: CFG, cfgToPdgNodeMap: map<CFGNode, PDGNode>) returns (E: set<PDGEdge>)
+{
 	E := {};
-	cfgNodes := set node | node in cfgToPdgNodeMap;
+	var cfgNodes := set node | node in cfgToPdgNodeMap;
 	while (|cfgNodes| > 0) 
 	invariant forall n :: n in cfgNodes ==> n in cfgToPdgNodeMap
 	{
@@ -62,6 +87,4 @@ method ComputePDG(S: Statement, cfg: CFG) returns (N: set<PDGNode>, E: set<PDGEd
 			case Exit =>
 		}
 	}
-		
 }
-
