SlideDG.dfy
@@ -10,13 +10,17 @@ type SlideDG = (Statement, set<Slide>, map<Slide, set<Slide>>) // map from node 
 
 method ComputeSlideDG(S: Statement, pdgN: set<PDGNode>, pdgE: set<PDGEdge>) returns (slideDG: SlideDG)
 	requires Core(S)
+	ensures SlideDGOf(slideDG, S)
 {
 	var N := ComputeSlideDGNodes(S, pdgN);
 	var E := ComputeSlideDGEdges(S, N);
 	var m : map<Slide, set<Slide>>; // TODO
 
-	//slideDG := (S, N, E, m);
+	slideDG := (S, N, m);
 }
+
+predicate SlideDGOf(slideDG: SlideDG, S: Statement)
+
 
 method ComputeSlideDGNodes(S: Statement, pdgN: set<PDGNode>) returns (slides: set<Slide>)
 	requires Core(S)
@@ -41,6 +45,39 @@ method ComputeSlideDGNodes(S: Statement, pdgN: set<PDGNode>) returns (slides: se
 		}
 	}
 }
+
+function SlideDGNodes(S: Statement, cfgN: set<CFGNode>) : set<Slide>
+{
+	//set slide | slide
+}
+
+
+// With CFG instead of PDG:
+
+/*method ComputeSlideDGNodes(S: Statement, cfgN: set<CFGNode>) returns (slides: set<Slide>)
+	requires Core(S)
+{
+	slides := {};
+	var copyCFGN := cfgN;
+
+	while (|copyCFGN| > 0)
+	{
+		var cfgNode :| cfgNode in copyCFGN;
+		copyCFGN := copyCFGN - {cfgNode};
+		match cfgNode {
+			case Entry =>
+			case Exit =>
+			case Node(l) => 
+				var subS := FindSubstatement(S, l);
+				match subS {
+					case Assignment(LHS,RHS) =>
+						var v: Variable;
+						var slide := ComputeSlide(S, v /* LHS? */, l);
+						slides := slides + {slide};
+				}
+		}
+	}
+}*/
 
 method ComputeSlideDGEdges(S: Statement, Slides: set<Slide>) returns (edges: set<Edge>)
 	requires Core(S)
@@ -75,3 +112,25 @@ method ComputeSlide(S: Statement, v: Variable, l: Label) returns (n: Slide)
 
 
 function SlideDGNeighbours(n: Slide) : set<Slide>
+
+function slidesOf(S: Statement, V: set<Variable>) : set<Slide>
+	reads *
+	requires Valid(S)
+	requires Core(S)
+{
+	slidesOf'(S, V, [], {})
+}
+
+function slidesOf'(S: Statement, V: set<Variable>, l: Label, nodes: set<CFGNode>) : set<Slide>
+	reads *
+	requires Valid(S)
+	requires Core(S)
+{
+	match S {
+	case Skip => {}
+	case Assignment(LHS,RHS) => set v | v in V * setOf(LHS) :: (CFGNode.Node(l), v, nodes)
+	case SeqComp(S1,S2) =>		slidesOf'(S1, V, l+[1], nodes) + slidesOf'(S2, V, l+[2], nodes)
+	case IF(B0,Sthen,Selse) =>	slidesOf'(Sthen, V, l+[1], nodes + {CFGNode.Node(l)}) + slidesOf'(Selse, V, l+[2], nodes + {CFGNode.Node(l)})
+	case DO(B,Sloop) =>			slidesOf'(Sloop, V, l+[1], nodes + {CFGNode.Node(l)})
+	}
+}
