VarSlideDG.dfy
@@ -1,0 +1,39 @@
+include "Definitions.dfy"
+include "Util.dfy"
+include "PDG.dfy"
+
+
+// VarSlideDG Definitions:
+datatype VarSlideTag = Phi | Regular
+type VarSlide = (Variable, VarSlideTag)
+type VarEdge = (VarSlide, VarSlide, set<Variable>)
+type VarSlideDG = (Statement, set<VarSlide>, map<VarSlide, set<VarSlide>>) // map from node to it's predecssors
+
+method ComputeVarSlideDG(S: Statement) returns (varSlideDG: VarSlideDG)
+	ensures VarSlideDGOf(varSlideDG, S)
+
+predicate VarSlideDGOf(varSlideDG: VarSlideDG, S: Statement)
+
+/*
+method ComputeVarSlideDG(S: Statement, pdgN: set<PDGNode>, pdgE: set<PDGEdge>) returns (varSlideDG: VarSlideDG)
+{
+	var N := ComputeVarSlideDGNodes(S, pdgN);
+	var E := ComputeVarSlideDGEdges(S, N);
+	var m : map<VarSlide, set<VarSlide>>; // TODO
+
+	//varSlideDG := (S, N, E, m);
+}
+
+method ComputeVarSlideDGNodes(S: Statement, pdgN: set<PDGNode>) returns (slides: set<VarSlide>)
+{
+
+}
+
+method ComputeVarSlideDGEdges(S: Statement, Slides: set<SSASlide>) returns (edges: set<VarEdge>)
+{
+
+}*/
+
+function varSlidesOf(S: Statement, V: set<Variable>) : set<VarSlide>
+
+predicate VarSlideDGReachable(from: VarSlide, to: VarSlide, S: set<VarSlide>)
